program_logic/hoare.v
@@ -29,12 +29,16 @@ Global Instance ht_mono' E :
   Proper (flip (⊑) ==> eq ==> pointwise_relation _ (⊑) ==> (⊑)) (@ht Λ Σ E).
 Proof. by intros P P' HP e ? <- Q Q' HQ; apply ht_mono. Qed.
 
+Lemma ht_alt E P Q e : (P ⊑ wp E e Q) → {{ P }} e @ E {{ Q }}.
+Proof.
+  intros; rewrite -{1}always_const. apply (always_intro _ _), impl_intro_l.
+  by rewrite always_const right_id.
+Qed.
+
 Lemma ht_val E v :
   {{ True : iProp Λ Σ }} of_val v @ E {{ λ v', v = v' }}.
-Proof.
-  apply (always_intro _ _), impl_intro_l.
-  by rewrite -wp_value'; apply const_intro.
-Qed.
+Proof. apply ht_alt. by rewrite -wp_value'; apply const_intro. Qed.
+
 Lemma ht_vs E P P' Q Q' e :
   ((P ={E}=> P') ∧ {{ P' }} e @ E {{ Q' }} ∧ ∀ v, Q' v ={E}=> Q v)
   ⊑ {{ P }} e @ E {{ Q }}.
@@ -45,6 +49,7 @@ Proof.
   rewrite -(pvs_wp E e Q) -(wp_pvs E e Q); apply pvs_mono, wp_mono=> v.
   by rewrite (forall_elim v) {1}/vs always_elim impl_elim_r.
 Qed.
+
 Lemma ht_atomic E1 E2 P P' Q Q' e :
   E2 ⊆ E1 → atomic e →
   ((P ={E1,E2}=> P') ∧ {{ P' }} e @ E2 {{ Q' }} ∧ ∀ v, Q' v ={E2,E1}=> Q v)
@@ -56,6 +61,7 @@ Proof.
   rewrite -(wp_atomic E1 E2) //; apply pvs_mono, wp_mono=> v.
   by rewrite (forall_elim v) {1}/vs always_elim impl_elim_r.
 Qed.
+
 Lemma ht_bind `{LanguageCtx Λ K} E P Q Q' e :
   ({{ P }} e @ E {{ Q }} ∧ ∀ v, {{ Q v }} K (of_val v) @ E {{ Q' }})
   ⊑ {{ P }} K e @ E {{ Q' }}.
@@ -65,9 +71,11 @@ Proof.
   rewrite wp_always_r -wp_bind //; apply wp_mono=> v.
   by rewrite (forall_elim v) /ht always_elim impl_elim_r.
 Qed.
+
 Lemma ht_mask_weaken E1 E2 P Q e :
   E1 ⊆ E2 → {{ P }} e @ E1 {{ Q }} ⊑ {{ P }} e @ E2 {{ Q }}.
 Proof. intros. by apply always_mono, impl_mono, wp_mask_frame_mono. Qed.
+
 Lemma ht_frame_l E P Q R e :
   {{ P }} e @ E {{ Q }} ⊑ {{ R ★ P }} e @ E {{ λ v, R ★ Q v }}.
 Proof.
@@ -75,9 +83,11 @@ Proof.
   rewrite always_and_sep_r -assoc (sep_and P) always_elim impl_elim_r.
   by rewrite wp_frame_l.
 Qed.
+
 Lemma ht_frame_r E P Q R e :
   {{ P }} e @ E {{ Q }} ⊑ {{ P ★ R }} e @ E {{ λ v, Q v ★ R }}.
 Proof. setoid_rewrite (comm _ _ R); apply ht_frame_l. Qed.
+
 Lemma ht_frame_later_l E P R e Q :
   to_val e = None →
   {{ P }} e @ E {{ Q }} ⊑ {{ ▷ R ★ P }} e @ E {{ λ v, R ★ Q v }}.
@@ -86,6 +96,7 @@ Proof.
   rewrite always_and_sep_r -assoc (sep_and P) always_elim impl_elim_r.
   by rewrite wp_frame_later_l //; apply wp_mono=>v; rewrite pvs_frame_l.
 Qed.
+
 Lemma ht_frame_later_r E P R e Q :
   to_val e = None →
   {{ P }} e @ E {{ Q }} ⊑ {{ P ★ ▷ R }} e @ E {{ λ v, Q v ★ R }}.
@@ -93,4 +104,5 @@ Proof.
   rewrite (comm _ _ (▷ R)%I); setoid_rewrite (comm _ _ R).
   apply ht_frame_later_l.
 Qed.
+
 End hoare.
